Another big cleanup - no more functions!

Bananas.thy
@@ -6,7 +6,6 @@ datatype type =
   Unit
 | Prod type type (infixr "\<otimes>" 80)
 | Sum type type (infixr "\<oplus>" 80)
-| Func type type (infixr "\<rightarrow>" 70)
 | \<mu> funct
 and funct =
   Id
@@ -20,166 +19,121 @@ primrec apply_functor :: "funct \<Rightarrow> type \<Rightarrow> type" (infixr "
 | "ProdF f\<^sub>1 f\<^sub>2 \<star> t = (f\<^sub>1 \<star> t) \<otimes> (f\<^sub>2 \<star> t)"
 | "SumF f\<^sub>1 f\<^sub>2 \<star> t = (f\<^sub>1 \<star> t) \<oplus> (f\<^sub>2 \<star> t)"
 
-datatype expr = 
-  Apply expr expr (infixl "\<cdot>" 70)
-| UnitV
-| PairV expr expr 
-| InlV expr
-| InrV expr
+datatype val = 
+  UnitV
+| PairV val val 
+| InlV val
+| InrV val
+| InjV funct val 
 
-| \<pi>\<^sub>1 
-| \<pi>\<^sub>2 
-| Tuple expr expr (infix "\<triangle>" 80)
-| \<iota>\<^sub>l 
-| \<iota>\<^sub>r 
-| Case expr expr (infix "\<nabla>" 80)
-| Inj funct expr 
+datatype expr = 
+  \<epsilon>
+| \<pi>\<^sub>1 | \<pi>\<^sub>2 | Tuple expr expr (infix "\<triangle>" 80)
+| \<iota>\<^sub>l | \<iota>\<^sub>r | Case expr expr (infix "\<nabla>" 80)
 | Outj funct
 
-inductive typecheck :: "expr \<Rightarrow> type \<Rightarrow> bool" (infix "\<turnstile>" 60) where
-  tc_app [simp]: "e\<^sub>1 \<turnstile> t\<^sub>1 \<rightarrow> t\<^sub>2 \<Longrightarrow> e\<^sub>2 \<turnstile> t\<^sub>1 \<Longrightarrow> e\<^sub>1 \<cdot> e\<^sub>2 \<turnstile> t\<^sub>2"
-| tc_unit [simp]: "UnitV \<turnstile> Unit"
-| tc_pair [simp]: "e\<^sub>1 \<turnstile> t\<^sub>1 \<Longrightarrow> e\<^sub>2 \<turnstile> t\<^sub>2 \<Longrightarrow> PairV e\<^sub>1 e\<^sub>2 \<turnstile> t\<^sub>1 \<otimes> t\<^sub>2"
-| tc_inlv [simp]: "e \<turnstile> t\<^sub>1 \<Longrightarrow> InlV e \<turnstile> t\<^sub>1 \<oplus> t\<^sub>2"
-| tc_inrv [simp]: "e \<turnstile> t\<^sub>2 \<Longrightarrow> InrV e \<turnstile> t\<^sub>1 \<oplus> t\<^sub>2"
+inductive typecheck\<^sub>v :: "val \<Rightarrow> type \<Rightarrow> bool" (infix "\<turnstile>" 60) where
+  tc_unit [simp]: "UnitV \<turnstile> Unit"
+| tc_pair [simp]: "v\<^sub>1 \<turnstile> t\<^sub>1 \<Longrightarrow> v\<^sub>2 \<turnstile> t\<^sub>2 \<Longrightarrow> PairV v\<^sub>1 v\<^sub>2 \<turnstile> t\<^sub>1 \<otimes> t\<^sub>2"
+| tc_inlv [simp]: "v \<turnstile> t\<^sub>1 \<Longrightarrow> InlV v \<turnstile> t\<^sub>1 \<oplus> t\<^sub>2"
+| tc_inrv [simp]: "v \<turnstile> t\<^sub>2 \<Longrightarrow> InrV v \<turnstile> t\<^sub>1 \<oplus> t\<^sub>2"
+| tc_inj [simp]: "v \<turnstile> f \<star> \<mu> f \<Longrightarrow> InjV f v \<turnstile> \<mu> f"
+
+inductive_cases [elim]: "UnitV \<turnstile> t"
+inductive_cases [elim]: "PairV e\<^sub>1 e\<^sub>2 \<turnstile> t"
+inductive_cases [elim]: "InrV e \<turnstile> t"
+inductive_cases [elim]: "InlV e \<turnstile> t"
+inductive_cases [elim]: "InjV f e \<turnstile> t"
+
+inductive typecheck\<^sub>e :: "expr \<Rightarrow> type \<Rightarrow> type \<Rightarrow> bool" (infix "\<turnstile> _ \<rightarrow>" 60) where
+  tc_id [simp]: "\<epsilon> \<turnstile> t \<rightarrow> t"
 | tc_fst [simp]: "\<pi>\<^sub>1 \<turnstile> t\<^sub>1 \<otimes> t\<^sub>2 \<rightarrow> t\<^sub>1"
 | tc_snd [simp]: "\<pi>\<^sub>2 \<turnstile> t\<^sub>1 \<otimes> t\<^sub>2 \<rightarrow> t\<^sub>2"
 | tc_tup [simp]: "f\<^sub>1 \<turnstile> t\<^sub>1 \<rightarrow> t\<^sub>2 \<Longrightarrow> f\<^sub>2 \<turnstile> t\<^sub>1 \<rightarrow> t\<^sub>3 \<Longrightarrow> f\<^sub>1 \<triangle> f\<^sub>2 \<turnstile> t\<^sub>1 \<rightarrow> t\<^sub>2 \<otimes> t\<^sub>3"
 | tc_inl [simp]: "\<iota>\<^sub>l \<turnstile> t\<^sub>1 \<rightarrow> t\<^sub>1 \<oplus> t\<^sub>2"
 | tc_inr [simp]: "\<iota>\<^sub>r \<turnstile> t\<^sub>2 \<rightarrow> t\<^sub>1 \<oplus> t\<^sub>2"
 | tc_case [simp]: "f\<^sub>l \<turnstile> t\<^sub>1 \<rightarrow> t\<^sub>3 \<Longrightarrow> f\<^sub>r \<turnstile> t\<^sub>2 \<rightarrow> t\<^sub>3 \<Longrightarrow> f\<^sub>l \<nabla> f\<^sub>r \<turnstile> t\<^sub>1 \<oplus> t\<^sub>2 \<rightarrow> t\<^sub>3"
-| tc_inj [simp]: "e \<turnstile> f \<star> \<mu> f \<Longrightarrow> Inj f e \<turnstile> \<mu> f"
 | tc_outj [simp]: "Outj f \<turnstile> \<mu> f \<rightarrow> f \<star> \<mu> f"
 
-inductive_cases [elim]: "e\<^sub>1 \<cdot> e\<^sub>2 \<turnstile> t"
-inductive_cases [elim]: "UnitV \<turnstile> t"
-inductive_cases [elim]: "PairV e\<^sub>1 e\<^sub>2 \<turnstile> t"
-inductive_cases [elim]: "InrV e \<turnstile> t"
-inductive_cases [elim]: "InlV e \<turnstile> t"
-inductive_cases [elim]: "\<pi>\<^sub>1 \<turnstile> t"
-inductive_cases [elim]: "\<pi>\<^sub>2 \<turnstile> t"
-inductive_cases [elim]: "f\<^sub>1 \<triangle> f\<^sub>2 \<turnstile> t"
-inductive_cases [elim]: "\<iota>\<^sub>l \<turnstile> t"
-inductive_cases [elim]: "\<iota>\<^sub>r \<turnstile> t"
-inductive_cases [elim]: "f\<^sub>l \<nabla> f\<^sub>r \<turnstile> t"
-inductive_cases [elim]: "Inj f e \<turnstile> t"
-inductive_cases [elim]: "Outj f \<turnstile> t"
+inductive_cases [elim]: "\<epsilon> \<turnstile> t \<rightarrow> t'"
+inductive_cases [elim]: "\<pi>\<^sub>1 \<turnstile> t \<rightarrow> t'"
+inductive_cases [elim]: "\<pi>\<^sub>2 \<turnstile> t \<rightarrow> t'"
+inductive_cases [elim]: "f\<^sub>1 \<triangle> f\<^sub>2 \<turnstile> t \<rightarrow> t'"
+inductive_cases [elim]: "\<iota>\<^sub>l \<turnstile> t \<rightarrow> t'"
+inductive_cases [elim]: "\<iota>\<^sub>r \<turnstile> t \<rightarrow> t'"
+inductive_cases [elim]: "f\<^sub>l \<nabla> f\<^sub>r \<turnstile> t \<rightarrow> t'"
+inductive_cases [elim]: "Outj f \<turnstile> t \<rightarrow> t'"
 
-fun is_value :: "expr \<Rightarrow> bool" where
-  "is_value (e\<^sub>1 \<cdot> e\<^sub>2) = False"
-| "is_value _ = True"
-
-inductive evaluate :: "expr \<Rightarrow> expr \<Rightarrow> bool" (infix "\<leadsto>" 60) where
-  ev_fun [simp]: "e\<^sub>1 \<leadsto> e\<^sub>1' \<Longrightarrow> e\<^sub>1 \<cdot> e\<^sub>2 \<leadsto> e\<^sub>1' \<cdot> e\<^sub>2"
-| ev_arg [simp]: "is_value e\<^sub>1 \<Longrightarrow> e\<^sub>2 \<leadsto> e\<^sub>2' \<Longrightarrow> e\<^sub>1 \<cdot> e\<^sub>2 \<leadsto> e\<^sub>1 \<cdot> e\<^sub>2'"
-| ev_fst [simp]: "\<pi>\<^sub>1 \<cdot> (PairV e\<^sub>1 e\<^sub>2) \<leadsto> e\<^sub>1"
-| ev_snd [simp]: "\<pi>\<^sub>2 \<cdot> (PairV e\<^sub>1 e\<^sub>2) \<leadsto> e\<^sub>2"
-| ev_tup [simp]: "f\<^sub>1 \<triangle> f\<^sub>2 \<cdot> e \<leadsto> PairV (f\<^sub>1 \<cdot> e) (f\<^sub>2 \<cdot> e)"
-| ev_inl [simp]: "\<iota>\<^sub>l \<cdot> e \<leadsto> InlV e"
-| ev_inr [simp]: "\<iota>\<^sub>r \<cdot> e \<leadsto> InrV e"
-| ev_csl [simp]: "f\<^sub>l \<nabla> f\<^sub>r \<cdot> (InlV e) \<leadsto> f\<^sub>l \<cdot> e"
-| ev_csr [simp]: "f\<^sub>l \<nabla> f\<^sub>r \<cdot> (InrV e) \<leadsto> f\<^sub>r \<cdot> e"
-| ev_out [simp]: "Outj f \<cdot> (Inj f e) \<leadsto> e"
+inductive evaluate :: "val \<Rightarrow> expr \<Rightarrow> val \<Rightarrow> bool" (infix "~ _ \<leadsto>" 60) where
+  ev_id [simp]: "v ~ \<epsilon> \<leadsto> v"
+| ev_fst [simp]: "PairV v\<^sub>1 v\<^sub>2 ~ \<pi>\<^sub>1 \<leadsto> v\<^sub>1"
+| ev_snd [simp]: "PairV v\<^sub>1 v\<^sub>2 ~ \<pi>\<^sub>2 \<leadsto> v\<^sub>2"
+| ev_tup [simp]: "v ~ f\<^sub>1 \<leadsto> v\<^sub>1 \<Longrightarrow> v ~ f\<^sub>2 \<leadsto> v\<^sub>2 \<Longrightarrow> v ~ f\<^sub>1 \<triangle> f\<^sub>2 \<leadsto> PairV v\<^sub>1 v\<^sub>2"
+| ev_inl [simp]: "v ~ \<iota>\<^sub>l \<leadsto> InlV v"
+| ev_inr [simp]: "v ~ \<iota>\<^sub>r \<leadsto> InrV v"
+| ev_csl [simp]: "v ~ f\<^sub>l \<leadsto> v' \<Longrightarrow> InlV v ~ f\<^sub>l \<nabla> f\<^sub>r \<leadsto> v'"
+| ev_csr [simp]: "v ~ f\<^sub>r \<leadsto> v' \<Longrightarrow> InrV v ~ f\<^sub>l \<nabla> f\<^sub>r \<leadsto> v'"
+| ev_out [simp]: "InjV f v ~ Outj f \<leadsto> v"
 
 (* safety *)
 
-abbreviation dne :: "expr \<Rightarrow> bool" where
-  "dne e \<equiv> (\<not> (\<exists>e'. e \<leadsto> e'))"
+theorem preservation: "v ~ e \<leadsto> v' \<Longrightarrow> e \<turnstile> t\<^sub>1 \<rightarrow> t\<^sub>2 \<Longrightarrow> v \<turnstile> t\<^sub>1 \<Longrightarrow> v' \<turnstile> t\<^sub>2"
+  by (induction v e v' arbitrary: t\<^sub>1 t\<^sub>2 rule: evaluate.induct) fastforce+
 
-lemma [simp]: "dne UnitV" using evaluate.simps by blast
-lemma [simp]: "dne (PairV e\<^sub>1 e\<^sub>2)" using evaluate.simps by blast
-lemma [simp]: "dne (InlV e)" using evaluate.simps by blast
-lemma [simp]: "dne (InrV e)" using evaluate.simps by blast
-lemma [simp]: "dne \<pi>\<^sub>1" using evaluate.simps by blast
-lemma [simp]: "dne \<pi>\<^sub>2" using evaluate.simps by blast
-lemma [simp]: "dne (f\<^sub>1 \<triangle> f\<^sub>2)" using evaluate.simps by blast
-lemma [simp]: "dne \<iota>\<^sub>l" using evaluate.simps by blast
-lemma [simp]: "dne \<iota>\<^sub>r" using evaluate.simps by blast
-lemma [simp]: "dne (f\<^sub>l \<nabla> f\<^sub>r)" using evaluate.simps by blast
-lemma [simp]: "dne (Inj f e)" using evaluate.simps by blast
-lemma [simp]: "dne (Outj f)" using evaluate.simps by blast
+lemma canonical_unit: "v \<turnstile> Unit \<Longrightarrow> v = UnitV"
+  by (induction v Unit rule: typecheck\<^sub>v.induct) simp_all
 
-theorem value_does_not_evaluate: "is_value e \<Longrightarrow> dne e"
-  by (induction e) simp_all
+lemma canonical_prod: "v \<turnstile> t\<^sub>1 \<otimes> t\<^sub>2 \<Longrightarrow> \<exists>v\<^sub>1 v\<^sub>2. v\<^sub>1 \<turnstile> t\<^sub>1 \<and> v\<^sub>2 \<turnstile> t\<^sub>2 \<and> v = PairV v\<^sub>1 v\<^sub>2"
+  by (induction v "Prod t\<^sub>1 t\<^sub>2" rule: typecheck\<^sub>v.induct) simp_all
 
-theorem preservation: "e \<leadsto> e' \<Longrightarrow> e \<turnstile> t \<Longrightarrow> e' \<turnstile> t"
-  proof (induction e e' arbitrary: t rule: evaluate.induct)
-  case (ev_fun e\<^sub>1 e\<^sub>1' e\<^sub>2)
-    then obtain tt where "e\<^sub>1 \<turnstile> tt \<rightarrow> t \<and> e\<^sub>2 \<turnstile> tt" by blast
-    moreover with ev_fun have "e\<^sub>1' \<turnstile> tt \<rightarrow> t" by simp
-    ultimately show ?case by auto
-  next case (ev_arg e\<^sub>1 e\<^sub>2 e\<^sub>2')
-    then obtain tt where "e\<^sub>1 \<turnstile> tt \<rightarrow> t \<and> e\<^sub>2 \<turnstile> tt" by blast
-    moreover with ev_arg have "e\<^sub>2' \<turnstile> tt" by simp
-    ultimately show ?case by auto
-  qed fastforce+
+lemma canonical_sum: "v \<turnstile> t\<^sub>1 \<oplus> t\<^sub>2 \<Longrightarrow> \<exists>v'. (v' \<turnstile> t\<^sub>1 \<and> v = InlV v') \<or> (v' \<turnstile> t\<^sub>2 \<and> v = InrV v')"
+  by (induction v "Sum t\<^sub>1 t\<^sub>2" rule: typecheck\<^sub>v.induct) simp_all
 
-lemma canonical_unit: "e \<turnstile> Unit \<Longrightarrow> is_value e \<Longrightarrow> e = UnitV"
-  by (induction e Unit rule: typecheck.induct) simp_all
+lemma canonical_mu: "v \<turnstile> \<mu> f \<Longrightarrow> \<exists>v'. v' \<turnstile> f \<star> \<mu> f \<and> v = InjV f v'"
+  by (induction v "\<mu> f" rule: typecheck\<^sub>v.induct) simp_all
 
-lemma canonical_prod: "e \<turnstile> t\<^sub>1 \<otimes> t\<^sub>2 \<Longrightarrow> is_value e \<Longrightarrow> \<exists>e\<^sub>1 e\<^sub>2. e = PairV e\<^sub>1 e\<^sub>2"
-  by (induction e "Prod t\<^sub>1 t\<^sub>2" rule: typecheck.induct) simp_all
-
-lemma canonical_sum: "e \<turnstile> t\<^sub>1 \<oplus> t\<^sub>2 \<Longrightarrow> is_value e \<Longrightarrow> \<exists>e'. e = InlV e' \<or> e = InrV e'"
-  by (induction e "Sum t\<^sub>1 t\<^sub>2" rule: typecheck.induct) simp_all
-
-lemma canonical_mu: "e \<turnstile> \<mu> f \<Longrightarrow> is_value e \<Longrightarrow> \<exists>e'. e = Inj f e'"
-  by (induction e "\<mu> f" rule: typecheck.induct) simp_all
-
-theorem progress: "e \<turnstile> t \<Longrightarrow> is_value e \<or> (\<exists>e'. e \<leadsto> e')"
-  proof (induction e t rule: typecheck.induct)
-  case (tc_app e\<^sub>1 t\<^sub>1 t\<^sub>2 e\<^sub>2)
+theorem progress: "e \<turnstile> t\<^sub>1 \<rightarrow> t\<^sub>2 \<Longrightarrow> v \<turnstile> t\<^sub>1 \<Longrightarrow> \<exists>v'. v ~ e \<leadsto> v'"
+  proof (induction e t\<^sub>1 t\<^sub>2 arbitrary: v rule: typecheck\<^sub>e.induct)
+  case tc_id
+    have "v ~ \<epsilon> \<leadsto> v" by simp
+    thus ?case by fastforce
+  next case tc_fst
+    then obtain v\<^sub>1 v\<^sub>2 where "v = PairV v\<^sub>1 v\<^sub>2" using canonical_prod by blast
+    hence "v ~ \<pi>\<^sub>1 \<leadsto> v\<^sub>1" by simp
+    thus ?case by fastforce
+  next case tc_snd
+    then obtain v\<^sub>1 v\<^sub>2 where "v = PairV v\<^sub>1 v\<^sub>2" using canonical_prod by blast
+    hence "v ~ \<pi>\<^sub>2 \<leadsto> v\<^sub>2" by simp
+    thus ?case by fastforce
+  next case (tc_tup f\<^sub>1 t\<^sub>1 t\<^sub>2 f\<^sub>2 t\<^sub>3)
+    then obtain v\<^sub>1 where "v ~ f\<^sub>1 \<leadsto> v\<^sub>1" by blast
+    moreover from tc_tup obtain v\<^sub>2 where "v ~ f\<^sub>2 \<leadsto> v\<^sub>2" by blast
+    ultimately have "v ~ f\<^sub>1 \<triangle> f\<^sub>2 \<leadsto> PairV v\<^sub>1 v\<^sub>2" by simp
+    thus ?case by fastforce
+  next case tc_inl
+    have "v ~ \<iota>\<^sub>l \<leadsto> InlV v" by simp
+    thus ?case by fastforce
+  next case tc_inr
+    have "v ~ \<iota>\<^sub>r \<leadsto> InrV v" by simp
+    thus ?case by fastforce
+  next case (tc_case f\<^sub>l t\<^sub>1 t\<^sub>3 f\<^sub>r t\<^sub>2)
+    then obtain v' where V: "(v' \<turnstile> t\<^sub>1 \<and> v = InlV v') \<or> (v' \<turnstile> t\<^sub>2 \<and> v = InrV v')" 
+      using canonical_sum by blast
     thus ?case
-      proof (cases "is_value e\<^sub>1")
-      case True note T = True
-        thus ?thesis
-          proof (cases "is_value e\<^sub>2")
-          case True
-            with tc_app T show ?thesis
-              proof (induction e\<^sub>1 "t\<^sub>1 \<rightarrow> t\<^sub>2" arbitrary: t\<^sub>1 t\<^sub>2 rule: typecheck.induct)
-              case tc_fst
-                then obtain e\<^sub>2\<^sub>1 e\<^sub>2\<^sub>2 where "e\<^sub>2 = PairV e\<^sub>2\<^sub>1 e\<^sub>2\<^sub>2" using canonical_prod by blast
-                moreover have "\<pi>\<^sub>1 \<cdot> PairV e\<^sub>2\<^sub>1 e\<^sub>2\<^sub>2 \<leadsto> e\<^sub>2\<^sub>1" by simp
-                ultimately show ?case by fastforce
-              next case tc_snd
-                then obtain e\<^sub>2\<^sub>1 e\<^sub>2\<^sub>2 where "e\<^sub>2 = PairV e\<^sub>2\<^sub>1 e\<^sub>2\<^sub>2" using canonical_prod by blast
-                moreover have "\<pi>\<^sub>2 \<cdot> PairV e\<^sub>2\<^sub>1 e\<^sub>2\<^sub>2 \<leadsto> e\<^sub>2\<^sub>2" by simp
-                ultimately show ?case by fastforce
-              next case (tc_tup f\<^sub>1 _ _ f\<^sub>2)
-                have "f\<^sub>1 \<triangle> f\<^sub>2 \<cdot> e\<^sub>2 \<leadsto> PairV (f\<^sub>1 \<cdot> e\<^sub>2) (f\<^sub>2 \<cdot> e\<^sub>2)" by simp
-                thus ?case by fastforce
-              next case tc_inl
-                have "\<iota>\<^sub>l \<cdot> e\<^sub>2 \<leadsto> InlV e\<^sub>2" by simp
-                thus ?case by fastforce
-              next case tc_inr
-                have "\<iota>\<^sub>r \<cdot> e\<^sub>2 \<leadsto> InrV e\<^sub>2" by simp
-                thus ?case by fastforce
-              next case (tc_case f\<^sub>l _ _ f\<^sub>r)
-                then obtain e' where E: "e\<^sub>2 = InlV e' \<or> e\<^sub>2 = InrV e'" using canonical_sum by blast
-                thus ?case
-                  proof (cases "e\<^sub>2 = InlV e'")
-                  case True
-                    moreover have "f\<^sub>l \<nabla> f\<^sub>r \<cdot> InlV e' \<leadsto> f\<^sub>l \<cdot> e'" by simp
-                    ultimately show ?thesis by fastforce
-                  next case False
-                    have "f\<^sub>l \<nabla> f\<^sub>r \<cdot> InrV e' \<leadsto> f\<^sub>r \<cdot> e'" by simp
-                    with False E show ?thesis by fastforce
-                  qed
-              next case (tc_outj f)
-                then obtain e' where "e\<^sub>2 = Inj f e'" using canonical_mu by blast
-                moreover have "Outj f \<cdot> Inj f e' \<leadsto> e'" by simp
-                ultimately show ?case by fastforce
-              qed simp_all
-          next case False
-            with tc_app obtain e\<^sub>2' where "e\<^sub>2 \<leadsto> e\<^sub>2'" by blast
-            with True have "e\<^sub>1 \<cdot> e\<^sub>2 \<leadsto> e\<^sub>1 \<cdot> e\<^sub>2'" by simp
-            thus ?thesis by auto
-          qed
+      proof (cases "v' \<turnstile> t\<^sub>1 \<and> v = InlV v'")
+      case True
+        with tc_case obtain v\<^sub>1 where "v' ~ f\<^sub>l \<leadsto> v\<^sub>1" by blast 
+        with True have "v ~ f\<^sub>l \<nabla> f\<^sub>r \<leadsto> v\<^sub>1" by simp
+        thus ?thesis by fastforce
       next case False
-        with tc_app obtain e\<^sub>1' where "e\<^sub>1 \<leadsto> e\<^sub>1'" by blast
-        hence "e\<^sub>1 \<cdot> e\<^sub>2 \<leadsto> e\<^sub>1' \<cdot> e\<^sub>2" by simp
-        thus ?thesis by auto
+        from tc_case False V obtain v\<^sub>2 where "v' ~ f\<^sub>r \<leadsto> v\<^sub>2" by blast 
+        with False V have "v ~ f\<^sub>l \<nabla> f\<^sub>r \<leadsto> v\<^sub>2" by auto
+        thus ?thesis by fastforce
       qed
-  qed simp_all
+  next case (tc_outj f)
+    then obtain v' where "v = InjV f v'" using canonical_mu by blast
+    hence "v ~ Outj f \<leadsto> v'" by simp
+    thus ?case by fastforce
+  qed
  
 end
